require mutable chain for resolved writes

fixtures/TypeChecker.ml
@@ -1047,16 +1047,6 @@ let place_resolved_write_direct_parent_b = function
                | None -> false)
 | _ -> false
 
-(** val place_resolved_write_shape_b : place -> bool **)
-
-let rec place_resolved_write_shape_b p =
-  if place_resolved_write_direct_parent_b p
-  then true
-  else (match p with
-        | PVar _ -> false
-        | PDeref q -> place_resolved_write_shape_b q
-        | PField (q, _) -> place_resolved_write_shape_b q)
-
 (** val place_suffix_path : place -> field_path **)
 
 let rec place_suffix_path = function
@@ -4462,6 +4452,26 @@ let sctx_lookup =
 
 let sctx_lookup_mut =
   ctx_lookup_mut
+
+(** val place_resolved_write_mutable_chain_b :
+    root_env -> sctx -> place -> bool **)
+
+let rec place_resolved_write_mutable_chain_b r _UU03a3_ p =
+  if place_resolved_write_direct_parent_b p
+  then true
+  else (match p with
+        | PDeref q ->
+          (&&) (place_resolved_write_mutable_chain_b r _UU03a3_ q)
+            (match place_resolved_write_target r q with
+             | Some x ->
+               (match sctx_lookup_mut x _UU03a3_ with
+                | Some m ->
+                  (match m with
+                   | MImmutable -> false
+                   | MMutable -> true)
+                | None -> false)
+             | None -> false)
+        | _ -> false)
 
 (** val check_make_closure_captures_sctx_base :
     global_env -> outlives_ctx -> sctx -> ident list -> param list -> ty list
@@ -8764,7 +8774,7 @@ let rec infer_core_env_state_fuel_roots fuel env _UU03a9_ n r _UU03a3_ e =
        | None ->
          (match infer_place_sctx env _UU03a3_ p with
           | Infer_ok t_old ->
-            if place_resolved_write_shape_b p
+            if place_resolved_write_mutable_chain_b r _UU03a3_ p
             then (match place_resolved_write_target r p with
                   | Some x ->
                     (match root_env_lookup x r with
@@ -8849,7 +8859,7 @@ let rec infer_core_env_state_fuel_roots fuel env _UU03a9_ n r _UU03a3_ e =
           | Infer_ok t_old ->
             if usage_eqb (ty_usage t_old) ULinear
             then Infer_err (ErrUsageMismatch ((ty_usage t_old), UAffine))
-            else if place_resolved_write_shape_b p
+            else if place_resolved_write_mutable_chain_b r _UU03a3_ p
                  then (match place_resolved_write_target r p with
                        | Some x ->
                          (match sctx_lookup_mut x _UU03a3_ with
@@ -11128,7 +11138,7 @@ let rec infer_core_env_state_fuel_roots_shadow_safe fuel env _UU03a9_ n r _UU03a
        | None ->
          (match infer_place_sctx env _UU03a3_ p with
           | Infer_ok t_old ->
-            if place_resolved_write_shape_b p
+            if place_resolved_write_mutable_chain_b r _UU03a3_ p
             then (match place_resolved_write_target r p with
                   | Some x ->
                     (match root_env_lookup x r with
@@ -11213,7 +11223,7 @@ let rec infer_core_env_state_fuel_roots_shadow_safe fuel env _UU03a9_ n r _UU03a
           | Infer_ok t_old ->
             if usage_eqb (ty_usage t_old) ULinear
             then Infer_err (ErrUsageMismatch ((ty_usage t_old), UAffine))
-            else if place_resolved_write_shape_b p
+            else if place_resolved_write_mutable_chain_b r _UU03a3_ p
                  then (match place_resolved_write_target r p with
                        | Some x ->
                          (match sctx_lookup_mut x _UU03a3_ with
